@prefix : <http://loop3d.org/GSO/ontology/2020/1/geologicprocess/ontology#> .
@prefix owl: <http://www.w3.org/2002/07/owl#> .
@prefix rdf: <http://www.w3.org/1999/02/22-rdf-syntax-ns#> .
@prefix xml: <http://www.w3.org/XML/1998/namespace> .
@prefix xsd: <http://www.w3.org/2001/XMLSchema#> .
@prefix rdfs: <http://www.w3.org/2000/01/rdf-schema#> .
@base <http://loop3d.org/GSO/ontology/2020/1/geologicprocess/ontology> .

<http://loop3d.org/GSO/ontology/2020/1/geologicprocess/ontology> rdf:type owl:Ontology ;
                                                                  owl:imports <http://loop3d.org/GSO/ontology/2020/1/common/ontology> ,
                                                                              <http://loop3d.org/GSO/ontology/2020/1/geology/ontology> ;
                                                                  rdfs:comment "This file contains terms and definitions from the 2016 SKOS-RDF version of the CGI Event Process vocabulary."@en ,
                                                                               "This scheme specifies concepts used to describe the geological processes that are associated with geological events, as defined by the IUGS Commission for Geoscience Information (CGI) Geoscience Terminology Working Group."@en ,
                                                                               "dct:creator--  CGI Geoscience Terminology Working Group, OWL adaptation by Stephen Richard for Loop3D project"@en ,
                                                                               "dct:date--  2016-06-15"@en ,
                                                                               "dct:modified-- 2019-12-04"@en ;
                                                                  rdfs:label "Geologic Process"@en .

#################################################################
#    Annotation properties
#################################################################

###  http://purl.org/dc/terms/source
<http://purl.org/dc/terms/source> rdf:type owl:AnnotationProperty .


###  http://www.w3.org/2002/07/owl#qualifiedCardinality
owl:qualifiedCardinality rdf:type owl:AnnotationProperty .


#################################################################
#    Classes
#################################################################

###  http://loop3d.org/GSO/ontology/2020/1/common/Pause
<http://loop3d.org/GSO/ontology/2020/1/common/Pause> rdf:type owl:Class .


###  http://loop3d.org/GSO/ontology/2020/1/common/Process
<http://loop3d.org/GSO/ontology/2020/1/common/Process> rdf:type owl:Class .


###  http://loop3d.org/GSO/ontology/2020/1/geologicprocess/Accretion
<http://loop3d.org/GSO/ontology/2020/1/geologicprocess/Accretion> rdf:type owl:Class ;
                                                                  rdfs:subClassOf <http://loop3d.org/GSO/ontology/2020/1/geologicprocess/Tectonic_Process> ,
                                                                                  <http://loop3d.org/GSO/ontology/2020/1/geology/Additive_Process> ;
                                                                  <http://purl.org/dc/terms/source> "Neuendorf, K.K.E, Mehl, J.P. & Jackson, J.A. (eds), 2005. Glossary of geology, 5th Edition. American Geological Institute, Alexandria, 779 p."@en ;
                                                                  rdfs:comment "The addition of material to a continent. Typically involves convergent or transform motion."@en ;
                                                                  rdfs:label "accretion"@en .


###  http://loop3d.org/GSO/ontology/2020/1/geologicprocess/Biological_Evolution
<http://loop3d.org/GSO/ontology/2020/1/geologicprocess/Biological_Evolution> rdf:type owl:Class ;
                                                                             rdfs:subClassOf <http://loop3d.org/GSO/ontology/2020/1/geologicprocess/Biological_Process> ;
                                                                             rdfs:label "Evolution"@en .


###  http://loop3d.org/GSO/ontology/2020/1/geologicprocess/Biological_Precipitation
<http://loop3d.org/GSO/ontology/2020/1/geologicprocess/Biological_Precipitation> rdf:type owl:Class ;
                                                                                 rdfs:subClassOf <http://loop3d.org/GSO/ontology/2020/1/geologicprocess/Deposition> ;
                                                                                 <http://purl.org/dc/terms/source> "this vocabulary"@en ;
                                                                                 rdfs:comment "The deposition of minerals from solution by the agency of organisms"@en ;
                                                                                 rdfs:label "biological precipitation"@en .


###  http://loop3d.org/GSO/ontology/2020/1/geologicprocess/Biological_Process
<http://loop3d.org/GSO/ontology/2020/1/geologicprocess/Biological_Process> rdf:type owl:Class ;
                                                                           rdfs:subClassOf <http://loop3d.org/GSO/ontology/2020/1/common/Process> ;
                                                                           rdfs:label "Biological Process"@en .


###  http://loop3d.org/GSO/ontology/2020/1/geologicprocess/Biological_Weathering
<http://loop3d.org/GSO/ontology/2020/1/geologicprocess/Biological_Weathering> rdf:type owl:Class ;
                                                                              rdfs:subClassOf <http://loop3d.org/GSO/ontology/2020/1/geologicprocess/Weathering> ;
                                                                              <http://purl.org/dc/terms/source> "Neuendorf, K.K.E, Mehl, J.P. & Jackson, J.A. (eds), 2005. Glossary of geology, 5th Edition. American Geological Institute, Alexandria, 779 p."@en ;
                                                                              rdfs:comment "breakdown of rocks by biological agents, e.g. the penetrating and expanding force of roots, the presence of moss and lichen causing humic acids to be retained in contact with rock, and the work of animals (worms, moles, rabbits) in modifying surface soil"@en ;
                                                                              rdfs:label "biological weathering"@en .


###  http://loop3d.org/GSO/ontology/2020/1/geologicprocess/Bolide_Impact
<http://loop3d.org/GSO/ontology/2020/1/geologicprocess/Bolide_Impact> rdf:type owl:Class ;
                                                                      rdfs:subClassOf <http://loop3d.org/GSO/ontology/2020/1/geology/Deformation> ;
                                                                      <http://purl.org/dc/terms/source> "Smulikowski et al, 2003"@en ;
                                                                      rdfs:comment "Metamorphism resulting from the passage of a shock wave through a body of material, typically the result of impact of a planetary body (impactor) on a planetary surface (target)"@en ;
                                                                      rdfs:label "impact process"@en .


###  http://loop3d.org/GSO/ontology/2020/1/geologicprocess/Cataclastic_Deformation
<http://loop3d.org/GSO/ontology/2020/1/geologicprocess/Cataclastic_Deformation> rdf:type owl:Class ;
                                                                                rdfs:subClassOf <http://loop3d.org/GSO/ontology/2020/1/geology/Deformation> ;
                                                                                <http://purl.org/dc/terms/source> "based on Neuendorf et al 2005"@en ;
                                                                                rdfs:comment "Brittle deformation processes, i.e. the formation and growth of fractures and frictional sliding along fracture surfaces."@en ;
                                                                                rdfs:label "cataclastic deformation"@en .


###  http://loop3d.org/GSO/ontology/2020/1/geologicprocess/Chemical_Precipitation
<http://loop3d.org/GSO/ontology/2020/1/geologicprocess/Chemical_Precipitation> rdf:type owl:Class ;
                                                                               rdfs:subClassOf <http://loop3d.org/GSO/ontology/2020/1/geologicprocess/Deposition> ,
                                                                                               <http://loop3d.org/GSO/ontology/2020/1/geologicprocess/Metamorphic_Process> ;
                                                                               <http://purl.org/dc/terms/source> "Neuendorf, K.K.E, Mehl, J.P. & Jackson, J.A. (eds), 2005. Glossary of geology, 5th Edition. American Geological Institute, Alexandria, 779 p."@en ;
                                                                               rdfs:comment "The deposition of mineral matter by precipitation from solution or as a result of chemical reactions. May be sedimentary or hydrothermal."@en ;
                                                                               rdfs:label "chemical precipitation"@en .


###  http://loop3d.org/GSO/ontology/2020/1/geologicprocess/Chemical_Weathering
<http://loop3d.org/GSO/ontology/2020/1/geologicprocess/Chemical_Weathering> rdf:type owl:Class ;
                                                                            rdfs:subClassOf <http://loop3d.org/GSO/ontology/2020/1/geologicprocess/Weathering> ;
                                                                            <http://purl.org/dc/terms/source> "Neuendorf, K.K.E, Mehl, J.P. & Jackson, J.A. (eds), 2005. Glossary of geology, 5th Edition. American Geological Institute, Alexandria, 779 p."@en ;
                                                                            rdfs:comment "The process of weathering by which chemical reactions (hydrolysishydration, oxidation, carbonation, ion exchange, and solution) transform rocks and minerals into new chemical combinations that are stable under conditions prevailing at or near the Earth's surface, e.g. the alteration of orthoclase to kaolinite."@en ;
                                                                            rdfs:label "chemical weathering"@en .


###  http://loop3d.org/GSO/ontology/2020/1/geologicprocess/Contact_Metamorphism
<http://loop3d.org/GSO/ontology/2020/1/geologicprocess/Contact_Metamorphism> rdf:type owl:Class ;
                                                                             rdfs:subClassOf <http://loop3d.org/GSO/ontology/2020/1/geologicprocess/Metamorphic_Process> ;
                                                                             <http://purl.org/dc/terms/source> "Neuendorf, K.K.E, Mehl, J.P. & Jackson, J.A. (eds), 2005. Glossary of geology, 5th Edition. American Geological Institute, Alexandria, 779 p."@en ;
                                                                             rdfs:comment "Metamorphism taking place in rocks at or near their contact with a genetically related body of igneous rock"@en ;
                                                                             rdfs:label "contact metamorphism"@en .


###  http://loop3d.org/GSO/ontology/2020/1/geologicprocess/Continental_Breakup
<http://loop3d.org/GSO/ontology/2020/1/geologicprocess/Continental_Breakup> rdf:type owl:Class ;
                                                                            rdfs:subClassOf <http://loop3d.org/GSO/ontology/2020/1/geologicprocess/Tectonic_Process> ,
                                                                                            <http://loop3d.org/GSO/ontology/2020/1/geology/Deformation> ;
                                                                            <http://purl.org/dc/terms/source> "this vocabulary"@en ;
                                                                            rdfs:comment "Fragmentation of a continental plate into two or more smaller plates, may involve rifting or strike slip faulting."@en ;
                                                                            rdfs:label "continental breakup"@en .


###  http://loop3d.org/GSO/ontology/2020/1/geologicprocess/Continental_Collision
<http://loop3d.org/GSO/ontology/2020/1/geologicprocess/Continental_Collision> rdf:type owl:Class ;
                                                                              rdfs:subClassOf <http://loop3d.org/GSO/ontology/2020/1/geologicprocess/Tectonic_Process> ,
                                                                                              <http://loop3d.org/GSO/ontology/2020/1/geology/Additive_Process> ,
                                                                                              <http://loop3d.org/GSO/ontology/2020/1/geology/Deformation> ;
                                                                              <http://purl.org/dc/terms/source> "this vocabulary"@en ;
                                                                              rdfs:comment "The amalgamation of two continental plates or blocks along a convergent margin."@en ;
                                                                              rdfs:label "continental collision"@en .


###  http://loop3d.org/GSO/ontology/2020/1/geologicprocess/Debris_Flow_Deposition
<http://loop3d.org/GSO/ontology/2020/1/geologicprocess/Debris_Flow_Deposition> rdf:type owl:Class ;
                                                                               rdfs:subClassOf <http://loop3d.org/GSO/ontology/2020/1/geologicprocess/Mechanical_Deposition> ;
                                                                               <http://purl.org/dc/terms/source> "Postma 1986 Geology v. 14 p291-294"@en ;
                                                                               rdfs:comment "Laminar high-concentration, generally cohesionless deposition process. Flow types included liquefied flow, fluidized flow, grain flow, traction carpet or modified grain flow."@en ;
                                                                               rdfs:label "debris flow deposition"@en .


###  http://loop3d.org/GSO/ontology/2020/1/geologicprocess/Deep_Water_Oxygen_Depletion
<http://loop3d.org/GSO/ontology/2020/1/geologicprocess/Deep_Water_Oxygen_Depletion> rdf:type owl:Class ;
                                                                                    rdfs:subClassOf <http://loop3d.org/GSO/ontology/2020/1/geology/Subtractive_Process> ;
                                                                                    rdfs:comment "" ;
                                                                                    rdfs:label "Deep Water Oxygen Depletion"@en .


###  http://loop3d.org/GSO/ontology/2020/1/geologicprocess/Deformation_Twinning
<http://loop3d.org/GSO/ontology/2020/1/geologicprocess/Deformation_Twinning> rdf:type owl:Class ;
                                                                             rdfs:subClassOf <http://loop3d.org/GSO/ontology/2020/1/geology/Transformation> ;
                                                                             <http://purl.org/dc/terms/source> "Neuendorf, K.K.E, Mehl, J.P. & Jackson, J.A. (eds), 2005. Glossary of geology, 5th Edition. American Geological Institute, Alexandria, 779 p."@en ;
                                                                             rdfs:comment "Deformation of a crystal by gliding to produce crystallographic twinning."@en ;
                                                                             rdfs:label "deformation twinning"@en .


###  http://loop3d.org/GSO/ontology/2020/1/geologicprocess/Deposition
<http://loop3d.org/GSO/ontology/2020/1/geologicprocess/Deposition> rdf:type owl:Class ;
                                                                   rdfs:subClassOf <http://loop3d.org/GSO/ontology/2020/1/geologicprocess/Rock_Forming_Process> ,
                                                                                   <http://loop3d.org/GSO/ontology/2020/1/geologicprocess/Sedimentary_Process> ,
                                                                                   <http://loop3d.org/GSO/ontology/2020/1/geology/Additive_Process> ;
                                                                   <http://purl.org/dc/terms/source> "Neuendorf, K.K.E, Mehl, J.P. & Jackson, J.A. (eds), 2005. Glossary of geology, 5th Edition. American Geological Institute, Alexandria, 779 p."@en ;
                                                                   rdfs:comment "Accumulation of material, the constructive process of accumulation of sedimentary particles, chemical precipitation of mineral matter from solution, or the accumulation of organic material on the death of plants and animals."@en ;
                                                                   rdfs:label "deposition"@en .


###  http://loop3d.org/GSO/ontology/2020/1/geologicprocess/Deposition_Hiatus
<http://loop3d.org/GSO/ontology/2020/1/geologicprocess/Deposition_Hiatus> rdf:type owl:Class ;
                                                                          rdfs:subClassOf <http://loop3d.org/GSO/ontology/2020/1/common/Pause> ,
                                                                                          <http://org.semanticweb.owlapi/error#Error1> ;
                                                                          rdfs:comment "Pause in a process of sediment accumulation. Use to indicate paraconformable boundaries."@en ;
                                                                          rdfs:label "Deposition Hiatus "@en .


###  http://loop3d.org/GSO/ontology/2020/1/geologicprocess/Diagenetic_Process
<http://loop3d.org/GSO/ontology/2020/1/geologicprocess/Diagenetic_Process> rdf:type owl:Class ;
                                                                           rdfs:subClassOf <http://loop3d.org/GSO/ontology/2020/1/geologicprocess/Rock_Forming_Process> ,
                                                                                           <http://loop3d.org/GSO/ontology/2020/1/geologicprocess/Sedimentary_Process> ,
                                                                                           <http://loop3d.org/GSO/ontology/2020/1/geology/Transformation> ;
                                                                           <http://purl.org/dc/terms/source> "Neuendorf, K.K.E, Mehl, J.P. & Jackson, J.A. (eds), 2005. Glossary of geology, 5th Edition. American Geological Institute, Alexandria, 779 p."@en ;
                                                                           rdfs:comment "Any chemical, physical, or biological process that affects a sedimentary EarthMaterial after initial deposition, and during or after lithification, exclusive of weathering and metamorphism. [adapt. Jackson, 1997] Example processes include compaction, cementation, authigenesis, replacement, leachinghydration, and bacterial action. Includes processes that are normal in the surficial or outer part of the earth’s crust [Jackson, 1997]. Changes in a deeply buried sedimentary rock may be continuous from diagenesis into recrystallization to form a metamorphic rock. Robertson [1999] defines the boundary between diagenesis and metamorphism in sedimentary rocks as follows: \\the boundary between diagenesis and metamorphism is somewhat arbitrary and strongly dependent on the rock types involved. For example changes take place in organic materials at lower temperatures than in rocks dominated by silicate minerals. In mudrocks, a white mica (illite) crystallinity value of less than 0.42D.2U obtained by X-ray diffraction analysis, is used to define the onset of metamorphism (Kisch, 1991). In this scheme, the first appearance of glaucophane, lawsonite, paragonite, prehnite, pumpellyite or stilpnomelane is taken to indicate the lower limit of metamorphism (Frey and Kisch, 1987, Bucher and Frey, 1994, Frey and Robinson, 1998). Most workers agree that such mineral growth starts at 150 ± 50° C in silicate rocks. Many rock types may show no change in mineralogy under these conditions and hence the recognition of the onset of metamorphism will vary with bulk composition.\\"@en ;
                                                                           rdfs:label "diagenetic process"@en .


###  http://loop3d.org/GSO/ontology/2020/1/geologicprocess/Diffusion_Creep
<http://loop3d.org/GSO/ontology/2020/1/geologicprocess/Diffusion_Creep> rdf:type owl:Class ;
                                                                        rdfs:subClassOf <http://loop3d.org/GSO/ontology/2020/1/geology/Transformation> ;
                                                                        <http://purl.org/dc/terms/source> "Neuendorf, K.K.E, Mehl, J.P. & Jackson, J.A. (eds), 2005. Glossary of geology, 5th Edition. American Geological Institute, Alexandria, 779 p."@en ;
                                                                        rdfs:comment "Grain-scale, ductile deformation accomplished by the motion of atoms through crystals, along grain boundaries, and through pore fluids."@en ;
                                                                        rdfs:label "diffusion creep"@en .


###  http://loop3d.org/GSO/ontology/2020/1/geologicprocess/Dislocation_Metamorphism
<http://loop3d.org/GSO/ontology/2020/1/geologicprocess/Dislocation_Metamorphism> rdf:type owl:Class ;
                                                                                 rdfs:subClassOf <http://loop3d.org/GSO/ontology/2020/1/geologicprocess/Metamorphic_Process> ;
                                                                                 <http://purl.org/dc/terms/source> "Neuendorf, K.K.E, Mehl, J.P. & Jackson, J.A. (eds), 2005. Glossary of geology, 5th Edition. American Geological Institute, Alexandria, 779 p."@en ;
                                                                                 rdfs:comment "Metamorphism concentrated along narrow belts of shearing or crushing without an appreciable rise in temperature"@en ;
                                                                                 rdfs:label "dislocation metamorphism"@en .


###  http://loop3d.org/GSO/ontology/2020/1/geologicprocess/Dissolution
<http://loop3d.org/GSO/ontology/2020/1/geologicprocess/Dissolution> rdf:type owl:Class ;
                                                                    rdfs:subClassOf <http://loop3d.org/GSO/ontology/2020/1/geologicprocess/Chemical_Weathering> ,
                                                                                    <http://loop3d.org/GSO/ontology/2020/1/geology/Subtractive_Process> ;
                                                                    <http://purl.org/dc/terms/source> "Neuendorf, K.K.E, Mehl, J.P. & Jackson, J.A. (eds), 2005. Glossary of geology, 5th Edition. American Geological Institute, Alexandria, 779 p."@en ;
                                                                    rdfs:comment "The process of dissolving into a homogenous solution, as when an acidic solution dissolves limestone. In karst, refers to the process of dissolving rock to produce landforms, in contrast to solution, the chemical product of dissolution."@en ;
                                                                    rdfs:label "dissolution"@en .


###  http://loop3d.org/GSO/ontology/2020/1/geologicprocess/Dissolution_Creep
<http://loop3d.org/GSO/ontology/2020/1/geologicprocess/Dissolution_Creep> rdf:type owl:Class ;
                                                                          rdfs:subClassOf <http://loop3d.org/GSO/ontology/2020/1/geology/Transformation> ;
                                                                          <http://purl.org/dc/terms/source> "Neuendorf, K.K.E, Mehl, J.P. & Jackson, J.A. (eds), 2005. Glossary of geology, 5th Edition. American Geological Institute, Alexandria, 779 p."@en ;
                                                                          rdfs:comment "Deformation by dissolution under the effects of differential stress and its transport to a new location by movement of fluid in the rock body."@en ;
                                                                          rdfs:label "dissolution creep"@en .


###  http://loop3d.org/GSO/ontology/2020/1/geologicprocess/Ductile_Flattening
<http://loop3d.org/GSO/ontology/2020/1/geologicprocess/Ductile_Flattening> rdf:type owl:Class ;
                                                                           rdfs:subClassOf <http://loop3d.org/GSO/ontology/2020/1/geologicprocess/Ductile_Flow> ;
                                                                           rdfs:comment "Also known as pure shear; a three-dimensional homogeneous flattening of a body (http://www.geology.sdsu.edu/visualstructure/vss/htm_hlp/pure_s.htm) accomodated by ductile deformation. It is an example of irrotational strain in which body is elongated in one direction while being shortened perpendicularly (https://en.wikipedia.org/wiki/Pure_shear)."@en ;
                                                                           rdfs:label "Ductile Flattening"@en .


###  http://loop3d.org/GSO/ontology/2020/1/geologicprocess/Ductile_Flow
<http://loop3d.org/GSO/ontology/2020/1/geologicprocess/Ductile_Flow> rdf:type owl:Class ;
                                                                     rdfs:subClassOf <http://loop3d.org/GSO/ontology/2020/1/geology/Deformation> ;
                                                                     <http://purl.org/dc/terms/source> "Neuendorf, K.K.E, Mehl, J.P. & Jackson, J.A. (eds), 2005. Glossary of geology, 5th Edition. American Geological Institute, Alexandria, 779 p."@en ;
                                                                     rdfs:comment "Deformation without apparent loss of continuity at the scale of observation."@en ;
                                                                     rdfs:label "ductile flow"@en .


###  http://loop3d.org/GSO/ontology/2020/1/geologicprocess/Ductile_Simple_Shear
<http://loop3d.org/GSO/ontology/2020/1/geologicprocess/Ductile_Simple_Shear> rdf:type owl:Class ;
                                                                             rdfs:subClassOf <http://loop3d.org/GSO/ontology/2020/1/geologicprocess/Ductile_Flow> ,
                                                                                             <http://loop3d.org/GSO/ontology/2020/1/geologicprocess/Shearing> ;
                                                                             rdfs:comment "Simple shear accomodated by ductile deformation. Simple sheare is a deformation in which parallel planes in a material remain parallel and maintain a constant distance, while translating relative to each other (https://en.wikipedia.org/wiki/Simple_shear)."@en ;
                                                                             rdfs:label "Ductile Simple Shear"@en .


###  http://loop3d.org/GSO/ontology/2020/1/geologicprocess/Effusive_Eruption
<http://loop3d.org/GSO/ontology/2020/1/geologicprocess/Effusive_Eruption> rdf:type owl:Class ;
                                                                          rdfs:subClassOf <http://loop3d.org/GSO/ontology/2020/1/geologicprocess/Eruption_Process> ;
                                                                          <http://purl.org/dc/terms/source> "Orton, G.J., 1996. Volcanic environments. 485-567 in Readingh.G. (ed.), Sedimentary Environments: Processes, Facies and Stratigraphy, Third Edition. Blackwell Science, Oxford"@en ;
                                                                          rdfs:comment "Eruptions characterized by low volatile content of the erupting magma relative to ambient pressure"@en ;
                                                                          rdfs:label "effusive eruption"@en .


###  http://loop3d.org/GSO/ontology/2020/1/geologicprocess/Erosion
<http://loop3d.org/GSO/ontology/2020/1/geologicprocess/Erosion> rdf:type owl:Class ;
                                                                rdfs:subClassOf <http://loop3d.org/GSO/ontology/2020/1/geologicprocess/Sedimentary_Process> ,
                                                                                <http://loop3d.org/GSO/ontology/2020/1/geology/Subtractive_Process> ;
                                                                <http://purl.org/dc/terms/source> "this vocabulary"@en ;
                                                                rdfs:comment "The process of disaggregation of rock and displacement of the resultant particles (sediment) usually by the agents of currents such as, wind, water, or ice by downward or down-slope movement in response to gravity or by living organisms (in the case of bioerosion)."@en ;
                                                                rdfs:label "erosion"@en .


###  http://loop3d.org/GSO/ontology/2020/1/geologicprocess/Eruption_Process
<http://loop3d.org/GSO/ontology/2020/1/geologicprocess/Eruption_Process> rdf:type owl:Class ;
                                                                         rdfs:subClassOf <http://loop3d.org/GSO/ontology/2020/1/geologicprocess/Magmatic_Process> ,
                                                                                         <http://loop3d.org/GSO/ontology/2020/1/geologicprocess/Rock_Forming_Process> ,
                                                                                         <http://loop3d.org/GSO/ontology/2020/1/geology/Additive_Process> ;
                                                                         <http://purl.org/dc/terms/source> "Neuendorf, K.K.E, Mehl, J.P. & Jackson, J.A. (eds), 2005. Glossary of geology, 5th Edition. American Geological Institute, Alexandria, 779 p."@en ;
                                                                         rdfs:comment "The ejection of volcanic materials (lava, pyroclasts, and volcanic gases) onto the Earth's surface, either from a central vent or from a fissure or group of fissures"@en ;
                                                                         rdfs:label "eruption"@en .


###  http://loop3d.org/GSO/ontology/2020/1/geologicprocess/Excavation
<http://loop3d.org/GSO/ontology/2020/1/geologicprocess/Excavation> rdf:type owl:Class ;
                                                                   rdfs:subClassOf <http://loop3d.org/GSO/ontology/2020/1/geologicprocess/Human_Activity> ,
                                                                                   <http://loop3d.org/GSO/ontology/2020/1/geology/Subtractive_Process> ;
                                                                   <http://purl.org/dc/terms/source> "this vocabulary"@en ;
                                                                   rdfs:comment "The removal of material by human activity, as in a mining operation"@en ;
                                                                   rdfs:label "excavation"@en .


###  http://loop3d.org/GSO/ontology/2020/1/geologicprocess/Extinction
<http://loop3d.org/GSO/ontology/2020/1/geologicprocess/Extinction> rdf:type owl:Class ;
                                                                   rdfs:subClassOf <http://loop3d.org/GSO/ontology/2020/1/geologicprocess/Biological_Process> ;
                                                                   <http://purl.org/dc/terms/source> "this vocabulary"@en ;
                                                                   rdfs:comment "Process of disappearance of a species or higher taxon, so that it no longer exists anywhere or in the subsequent fossil record."@en ;
                                                                   rdfs:label "extinction"@en .


###  http://loop3d.org/GSO/ontology/2020/1/geologicprocess/Faulting
<http://loop3d.org/GSO/ontology/2020/1/geologicprocess/Faulting> rdf:type owl:Class ;
                                                                 rdfs:subClassOf <http://loop3d.org/GSO/ontology/2020/1/geology/Deformation> ;
                                                                 <http://purl.org/dc/terms/source> "Neuendorf, K.K.E, Mehl, J.P. & Jackson, J.A. (eds), 2005. Glossary of geology, 5th Edition. American Geological Institute, Alexandria, 779 p."@en ;
                                                                 rdfs:comment "The process of fracturing, frictional slip, and displacement accumulation that produces a fault"@en ;
                                                                 rdfs:label "faulting"@en .


###  http://loop3d.org/GSO/ontology/2020/1/geologicprocess/Flexural_Slip
<http://loop3d.org/GSO/ontology/2020/1/geologicprocess/Flexural_Slip> rdf:type owl:Class ;
                                                                      rdfs:subClassOf <http://loop3d.org/GSO/ontology/2020/1/geologicprocess/Folding> ;
                                                                      rdfs:comment "A folding process in which shearing is concentrated as layer boundaries and the folded layers maintain a relatively constant thickness"@en ;
                                                                      rdfs:isDefinedBy "this vocabulary"@en ;
                                                                      rdfs:label "Flexural slip folding @en}" .


###  http://loop3d.org/GSO/ontology/2020/1/geologicprocess/Folding
<http://loop3d.org/GSO/ontology/2020/1/geologicprocess/Folding> rdf:type owl:Class ;
                                                                rdfs:subClassOf <http://loop3d.org/GSO/ontology/2020/1/geology/Deformation> ;
                                                                <http://purl.org/dc/terms/source> "this vocabulary"@en ;
                                                                rdfs:comment "Deformation in which planar surfaces become regularly curviplanar surfaces with definable limbs (zones of lower curvature) and hinges (zones of higher curvature)."@en ;
                                                                rdfs:label "folding"@en .


###  http://loop3d.org/GSO/ontology/2020/1/geologicprocess/Fracturing
<http://loop3d.org/GSO/ontology/2020/1/geologicprocess/Fracturing> rdf:type owl:Class ;
                                                                   rdfs:subClassOf <http://loop3d.org/GSO/ontology/2020/1/geology/Deformation> ;
                                                                   <http://purl.org/dc/terms/source> "this vocabulary"@en ;
                                                                   rdfs:comment "The formation of a surface of failure resulting from stress"@en ;
                                                                   rdfs:label "fracturing"@en .


###  http://loop3d.org/GSO/ontology/2020/1/geologicprocess/Frost_Shattering
<http://loop3d.org/GSO/ontology/2020/1/geologicprocess/Frost_Shattering> rdf:type owl:Class ;
                                                                         rdfs:subClassOf <http://loop3d.org/GSO/ontology/2020/1/geologicprocess/Physical_Weathering> ;
                                                                         <http://purl.org/dc/terms/source> "Neuendorf, K.K.E, Mehl, J.P. & Jackson, J.A. (eds), 2005. Glossary of geology, 5th Edition. American Geological Institute, Alexandria, 779 p."@en ;
                                                                         rdfs:comment "Propagation of fractures due to expansion of freezing water in intergranular spaces and fractures in a rock body. Result is mechanical disintegration spliitting, or breakup of rock."@en ;
                                                                         rdfs:label "frost shattering"@en .


###  http://loop3d.org/GSO/ontology/2020/1/geologicprocess/Geodynamo_Process
<http://loop3d.org/GSO/ontology/2020/1/geologicprocess/Geodynamo_Process> rdf:type owl:Class ;
                                                                          rdfs:subClassOf <http://loop3d.org/GSO/ontology/2020/1/geologicprocess/Geomagnetic_Process> ;
                                                                          rdfs:comment "Process that generates electric currents due to the motion of convection currents of molten iron in the Earth's outer core, caused by heat escaping from the core. Process responsible for Earth’s magnetic field."@en ;
                                                                          rdfs:label "Geodynamo process"@en .


###  http://loop3d.org/GSO/ontology/2020/1/geologicprocess/Geomagnetic_Process
<http://loop3d.org/GSO/ontology/2020/1/geologicprocess/Geomagnetic_Process> rdf:type owl:Class ;
                                                                            rdfs:subClassOf <http://loop3d.org/GSO/ontology/2020/1/common/Process> ;
                                                                            <http://purl.org/dc/terms/source> "this vocabulary"@en ;
                                                                            rdfs:comment "process that results in change in Earth's magnetic field"@en ;
                                                                            rdfs:label "Geomagnetic Process"@en .


###  http://loop3d.org/GSO/ontology/2020/1/geologicprocess/Grading
<http://loop3d.org/GSO/ontology/2020/1/geologicprocess/Grading> rdf:type owl:Class ;
                                                                rdfs:subClassOf <http://loop3d.org/GSO/ontology/2020/1/geologicprocess/Human_Activity> ,
                                                                                <http://loop3d.org/GSO/ontology/2020/1/geology/Transformation> ;
                                                                <http://purl.org/dc/terms/source> "this vocabulary"@en ;
                                                                rdfs:comment "Leveling of earth surface by rearrangement of prexisting material"@en ;
                                                                rdfs:label "grading"@en .


###  http://loop3d.org/GSO/ontology/2020/1/geologicprocess/Haloclasty
<http://loop3d.org/GSO/ontology/2020/1/geologicprocess/Haloclasty> rdf:type owl:Class ;
                                                                   rdfs:subClassOf <http://loop3d.org/GSO/ontology/2020/1/geologicprocess/Physical_Weathering> ;
                                                                   <http://purl.org/dc/terms/source> "Neuendorf, K.K.E, Mehl, J.P. & Jackson, J.A. (eds), 2005. Glossary of geology, 5th Edition. American Geological Institute, Alexandria, 779 p."@en ;
                                                                   rdfs:comment "Propagation of fractures in rock due to crytallization of mineral salts (typically sodium chloride) from interstitial water, or volumetrick expansion of salts in capillaries, or hydration pressure of interstitial, trapped salts. Generally results in mechanical disintegration of the rock surface."@en ;
                                                                   rdfs:label "haloclasty"@en .


###  http://loop3d.org/GSO/ontology/2020/1/geologicprocess/Hawaiian_Eruption
<http://loop3d.org/GSO/ontology/2020/1/geologicprocess/Hawaiian_Eruption> rdf:type owl:Class ;
                                                                          rdfs:subClassOf <http://loop3d.org/GSO/ontology/2020/1/geologicprocess/Eruption_Process> ;
                                                                          <http://purl.org/dc/terms/source> "Neuendorf, K.K.E, Mehl, J.P. & Jackson, J.A. (eds), 2005. Glossary of geology, 5th Edition. American Geological Institute, Alexandria, 779 p."@en ;
                                                                          rdfs:comment "Eruption in which great quantities of extremely fluid basaltic lava are poured out, mainly issuing in lava fountains from fissures on the flanks of a volcano. Explosive phenomena are rare, but much spatter and scoria are piled into cones and mounds along the vents. Characteristic of shield volcanoes"@en ;
                                                                          rdfs:label "hawaiian eruption"@en .


###  http://loop3d.org/GSO/ontology/2020/1/geologicprocess/Human_Activity
<http://loop3d.org/GSO/ontology/2020/1/geologicprocess/Human_Activity> rdf:type owl:Class ;
                                                                       rdfs:subClassOf <http://loop3d.org/GSO/ontology/2020/1/common/Process> ;
                                                                       <http://purl.org/dc/terms/source> "this vocabulary"@en ;
                                                                       rdfs:comment "Processes of human modification of the earth to produce geologic features"@en ;
                                                                       rdfs:label "Human Activity"@en .


###  http://loop3d.org/GSO/ontology/2020/1/geologicprocess/Human_Deposition
<http://loop3d.org/GSO/ontology/2020/1/geologicprocess/Human_Deposition> rdf:type owl:Class ;
                                                                         rdfs:subClassOf <http://loop3d.org/GSO/ontology/2020/1/geologicprocess/Human_Activity> ,
                                                                                         <http://loop3d.org/GSO/ontology/2020/1/geologicprocess/Mechanical_Deposition> ,
                                                                                         <http://loop3d.org/GSO/ontology/2020/1/geologicprocess/Rock_Forming_Process> ;
                                                                         rdfs:comment "Human processes of material deposition, e.g. landfill, mining waste heaps, tailings, road-grade fill."@en ;
                                                                         rdfs:label "Human material deposition "@en .


###  http://loop3d.org/GSO/ontology/2020/1/geologicprocess/Hydration
<http://loop3d.org/GSO/ontology/2020/1/geologicprocess/Hydration> rdf:type owl:Class ;
                                                                  rdfs:subClassOf <http://loop3d.org/GSO/ontology/2020/1/geologicprocess/Chemical_Weathering> ;
                                                                  <http://purl.org/dc/terms/source> "this vocabulary"@en ;
                                                                  rdfs:comment "The process of absorption of water into the crystal structure of a mineral, thereby changing its volume and fracturing and loosening grains"@en ;
                                                                  rdfs:label "hydration"@en .


###  http://loop3d.org/GSO/ontology/2020/1/geologicprocess/Hydrolysis
<http://loop3d.org/GSO/ontology/2020/1/geologicprocess/Hydrolysis> rdf:type owl:Class ;
                                                                   rdfs:subClassOf <http://loop3d.org/GSO/ontology/2020/1/geologicprocess/Chemical_Weathering> ;
                                                                   <http://purl.org/dc/terms/source> "Neuendorf, K.K.E, Mehl, J.P. & Jackson, J.A. (eds), 2005. Glossary of geology, 5th Edition. American Geological Institute, Alexandria, 779 p."@en ;
                                                                   rdfs:comment "A decomposition reaction involving water. In geology, it commonly indicates reaction between silicate minerals and either pure water or aqueous solution. In such reactionsh"@en ;
                                                                   rdfs:label "hydrolysis"@en .


###  http://loop3d.org/GSO/ontology/2020/1/geologicprocess/Ice_Erosion
<http://loop3d.org/GSO/ontology/2020/1/geologicprocess/Ice_Erosion> rdf:type owl:Class ;
                                                                    rdfs:subClassOf <http://loop3d.org/GSO/ontology/2020/1/geologicprocess/Erosion> ;
                                                                    <http://purl.org/dc/terms/source> "this vocabulary"@en ;
                                                                    rdfs:comment "Erosion by corrasion or plucking by moving ice."@en ;
                                                                    rdfs:label "ice erosion"@en .


###  http://loop3d.org/GSO/ontology/2020/1/geologicprocess/Intrusion_Process
<http://loop3d.org/GSO/ontology/2020/1/geologicprocess/Intrusion_Process> rdf:type owl:Class ;
                                                                          rdfs:subClassOf <http://loop3d.org/GSO/ontology/2020/1/geology/Additive_Process> ;
                                                                          <http://purl.org/dc/terms/source> "Neuendorf, K.K.E, Mehl, J.P. & Jackson, J.A. (eds), 2005. Glossary of geology, 5th Edition. American Geological Institute, Alexandria, 779 p."@en ;
                                                                          rdfs:comment "The process of emplacement of magma in pre-existing rock"@en ;
                                                                          rdfs:label "intrusion"@en .


###  http://loop3d.org/GSO/ontology/2020/1/geologicprocess/Lava_Flow
<http://loop3d.org/GSO/ontology/2020/1/geologicprocess/Lava_Flow> rdf:type owl:Class ;
                                                                  rdfs:subClassOf <http://loop3d.org/GSO/ontology/2020/1/geologicprocess/Eruption_Process> ;
                                                                  rdfs:comment "process of melted rock flowing over the Earth's surface and solidifying to form new rock."@en ;
                                                                  rdfs:label "Lava Flow "@en .


###  http://loop3d.org/GSO/ontology/2020/1/geologicprocess/Magmatic_Cystallisation
<http://loop3d.org/GSO/ontology/2020/1/geologicprocess/Magmatic_Cystallisation> rdf:type owl:Class ;
                                                                                rdfs:subClassOf <http://loop3d.org/GSO/ontology/2020/1/geologicprocess/Magmatic_Process> ,
                                                                                                <http://loop3d.org/GSO/ontology/2020/1/geologicprocess/Rock_Forming_Process> ,
                                                                                                <http://loop3d.org/GSO/ontology/2020/1/geology/Transformation> ;
                                                                                <http://purl.org/dc/terms/source> "Neuendorf, K.K.E, Mehl, J.P. & Jackson, J.A. (eds), 2005. Glossary of geology, 5th Edition. American Geological Institute, Alexandria, 779 p."@en ;
                                                                                rdfs:comment "The process by which matter becomes crystalline, from a gaseous, fluid, or dispersed state"@en ;
                                                                                rdfs:label "magmatic crystallisation"@en .


###  http://loop3d.org/GSO/ontology/2020/1/geologicprocess/Magmatic_Process
<http://loop3d.org/GSO/ontology/2020/1/geologicprocess/Magmatic_Process> rdf:type owl:Class ;
                                                                         rdfs:subClassOf <http://loop3d.org/GSO/ontology/2020/1/geology/Geologic_Process> ;
                                                                         <http://purl.org/dc/terms/source> "this vocabulary"@en ;
                                                                         rdfs:comment "A process involving melted rock (magma)."@en ;
                                                                         rdfs:label "Magmatic Process"@en .


###  http://loop3d.org/GSO/ontology/2020/1/geologicprocess/Mass_Wasting
<http://loop3d.org/GSO/ontology/2020/1/geologicprocess/Mass_Wasting> rdf:type owl:Class ;
                                                                     rdfs:subClassOf <http://loop3d.org/GSO/ontology/2020/1/geologicprocess/Erosion> ;
                                                                     <http://purl.org/dc/terms/source> "Neuendorf, K.K.E, Mehl, J.P. & Jackson, J.A. (eds), 2005. Glossary of geology, 5th Edition. American Geological Institute, Alexandria, 779 p."@en ;
                                                                     rdfs:comment "the dislodgement and downslope transport of soil and rock material under the direct application of gravitational body stresses. In contrast to other erosion processes, the debris removed by mass wasting is not carried within, on, or under another medium. The mass properties of the material being transported depend on the interaction of the soil and rock particles and on the moisture content."@en ;
                                                                     rdfs:label "mass wasting"@en .


###  http://loop3d.org/GSO/ontology/2020/1/geologicprocess/Mass_Wasting_Deposition
<http://loop3d.org/GSO/ontology/2020/1/geologicprocess/Mass_Wasting_Deposition> rdf:type owl:Class ;
                                                                                rdfs:subClassOf <http://loop3d.org/GSO/ontology/2020/1/geologicprocess/Mechanical_Deposition> ;
                                                                                <http://purl.org/dc/terms/source> "Neuendorf, K.K.E, Mehl, J.P. & Jackson, J.A. (eds), 2005. Glossary of geology, 5th Edition. American Geological Institute, Alexandria, 779 p."@en ;
                                                                                rdfs:comment "A general term for the dislodgement and downslope transport of soil and rock material under the direct application of gravitational body stresses. In contrast to other erosion processes, the debris removed by mass wasting is not carried within, on, or under another medium. The mass properties of the material being transported depend on the interaction of the soil and rock particles and on the moisture content. Mass wasting includes slow displacements, such as creep and solifluction, and rapid movements such as rockfalls, rockslides, and cohesive debris flows (Jackson, 1997, p. 392). Includes both subaerial mass-wasting processes and subaqueous mass-wasting processes."@en ;
                                                                                rdfs:label "mass wasting deposition"@en .


###  http://loop3d.org/GSO/ontology/2020/1/geologicprocess/Material_Transport
<http://loop3d.org/GSO/ontology/2020/1/geologicprocess/Material_Transport> rdf:type owl:Class ;
                                                                           rdfs:subClassOf <http://loop3d.org/GSO/ontology/2020/1/common/Process> ;
                                                                           <http://purl.org/dc/terms/source> "this vocabulary"@en ;
                                                                           rdfs:comment "Transport and heaping of material, as in a land fill, mine dump, dredging operations. Can be anthropogenic, or geologic transport process"@en ;
                                                                           rdfs:label "Material Transport And Deposition"@en .


###  http://loop3d.org/GSO/ontology/2020/1/geologicprocess/Mechanical_Deposition
<http://loop3d.org/GSO/ontology/2020/1/geologicprocess/Mechanical_Deposition> rdf:type owl:Class ;
                                                                              rdfs:subClassOf <http://loop3d.org/GSO/ontology/2020/1/geologicprocess/Deposition> ;
                                                                              <http://purl.org/dc/terms/source> "NADM SLTTs 2004"@en ;
                                                                              rdfs:comment "Process by which material that is being transported as particles by moving air, water, ice, or other fluid comes to rest and accumulates."@en ;
                                                                              rdfs:label "mechanical deposition"@en .


###  http://loop3d.org/GSO/ontology/2020/1/geologicprocess/Melting
<http://loop3d.org/GSO/ontology/2020/1/geologicprocess/Melting> rdf:type owl:Class ;
                                                                rdfs:subClassOf <http://loop3d.org/GSO/ontology/2020/1/geologicprocess/Magmatic_Process> ,
                                                                                <http://loop3d.org/GSO/ontology/2020/1/geology/Subtractive_Process> ,
                                                                                <http://loop3d.org/GSO/ontology/2020/1/geology/Transformation> ;
                                                                <http://purl.org/dc/terms/source> "this vocabulary"@en ;
                                                                rdfs:comment "change of state from a solid to a liquid"@en ;
                                                                rdfs:label "melting"@en .


###  http://loop3d.org/GSO/ontology/2020/1/geologicprocess/Metamorphic_Process
<http://loop3d.org/GSO/ontology/2020/1/geologicprocess/Metamorphic_Process> rdf:type owl:Class ;
                                                                            rdfs:subClassOf <http://loop3d.org/GSO/ontology/2020/1/geology/Transformation> ;
                                                                            <http://purl.org/dc/terms/source> "this vocabulary"@en ;
                                                                            rdfs:comment "Mineralogical, chemical, and structural adjustment of solid rocks to physical and chemical conditions that differ from the conditions under which the rocks in question originated, and are generally been imposed at depth, below the surface zones of weathering and cementation."@en ;
                                                                            rdfs:label "Metamorphic Process"@en .


###  http://loop3d.org/GSO/ontology/2020/1/geologicprocess/Metasomatism
<http://loop3d.org/GSO/ontology/2020/1/geologicprocess/Metasomatism> rdf:type owl:Class ;
                                                                     rdfs:subClassOf <http://loop3d.org/GSO/ontology/2020/1/geologicprocess/Metamorphic_Process> ;
                                                                     <http://purl.org/dc/terms/source> "Fettes and Desmons, 2007"@en ;
                                                                     rdfs:comment "Processes causing open-system changes in chemical composition by reaction with an external source, typically involving chemical transport by a fluid medium flowing through the rock. Metasomatism typically involves introduction of chemical constituents into a rock volume. General term for any change in the mineralogical or chemical composition of a rock. Typically related to interaction with hydrous fluids."@en ;
                                                                     rdfs:label "Metasomatism or hydrothermal process"@en .


###  http://loop3d.org/GSO/ontology/2020/1/geologicprocess/Microfracturing
<http://loop3d.org/GSO/ontology/2020/1/geologicprocess/Microfracturing> rdf:type owl:Class ;
                                                                        rdfs:subClassOf <http://loop3d.org/GSO/ontology/2020/1/geologicprocess/Fracturing> ;
                                                                        <http://purl.org/dc/terms/source> "Neuendorf, K.K.E, Mehl, J.P. & Jackson, J.A. (eds), 2005. Glossary of geology, 5th Edition. American Geological Institute, Alexandria, 779 p."@en ;
                                                                        rdfs:comment "Development of fractures within a single grain or cutting several grains."@en ;
                                                                        rdfs:label "microfracturing"@en .


###  http://loop3d.org/GSO/ontology/2020/1/geologicprocess/Mountain_Building
<http://loop3d.org/GSO/ontology/2020/1/geologicprocess/Mountain_Building> rdf:type owl:Class ;
                                                                          rdfs:subClassOf <http://loop3d.org/GSO/ontology/2020/1/geologicprocess/Tectonic_Process> ,
                                                                                          <http://loop3d.org/GSO/ontology/2020/1/geology/Deformation> ;
                                                                          <http://purl.org/dc/terms/source> "Neuendorf et al., 2005"@en ;
                                                                          rdfs:comment "orogenic process or mountain building process."@en ,
                                                                                       "skos:altLabel--  orogenesis"@en ;
                                                                          rdfs:label "Mountain building"@en .


###  http://loop3d.org/GSO/ontology/2020/1/geologicprocess/Obduction
<http://loop3d.org/GSO/ontology/2020/1/geologicprocess/Obduction> rdf:type owl:Class ;
                                                                  rdfs:subClassOf <http://loop3d.org/GSO/ontology/2020/1/geologicprocess/Tectonic_Process> ,
                                                                                  <http://loop3d.org/GSO/ontology/2020/1/geology/Deformation> ;
                                                                  <http://purl.org/dc/terms/source> "Neuendorf et al., 2005, http://en.wikipedia.org/wiki/Obduction, Coleman, R. G., 1971, Plate tectonic emplacement of upper mantle peridotites along continental edge: J.Geophys. Res., v75, p1212-1222."@en ;
                                                                  rdfs:comment "The overthrusting of continental crust by oceanic crust or mantle rocks at a convergent plate boundary."@en ;
                                                                  rdfs:label "obduction"@en .


###  http://loop3d.org/GSO/ontology/2020/1/geologicprocess/Organic_Accumulation
<http://loop3d.org/GSO/ontology/2020/1/geologicprocess/Organic_Accumulation> rdf:type owl:Class ;
                                                                             rdfs:subClassOf <http://loop3d.org/GSO/ontology/2020/1/geologicprocess/Deposition> ;
                                                                             rdfs:comment "Sediment accumulation of biologically produced organic material, as in bog, coal swamps."@en ;
                                                                             rdfs:label "organic accumulation"@en .


###  http://loop3d.org/GSO/ontology/2020/1/geologicprocess/Oxidation
<http://loop3d.org/GSO/ontology/2020/1/geologicprocess/Oxidation> rdf:type owl:Class ;
                                                                  rdfs:subClassOf <http://loop3d.org/GSO/ontology/2020/1/geologicprocess/Chemical_Weathering> ;
                                                                  <http://purl.org/dc/terms/source> "this vocabulary"@en ;
                                                                  rdfs:comment "Chemical reaction that involve stripping of electrons from cations. Typicall reactions include converting sulfide minerals to oxide minerals, or increasing the oxidation state of cations in existing oxide minerals. The most commonly observed is the oxidation of Fe"@en ;
                                                                  rdfs:label "oxidation"@en .


###  http://loop3d.org/GSO/ontology/2020/1/geologicprocess/Partial_Melting
<http://loop3d.org/GSO/ontology/2020/1/geologicprocess/Partial_Melting> rdf:type owl:Class ;
                                                                        rdfs:subClassOf <http://loop3d.org/GSO/ontology/2020/1/geologicprocess/Melting> ;
                                                                        <http://purl.org/dc/terms/source> "Neuendorf, K.K.E, Mehl, J.P. & Jackson, J.A. (eds), 2005. Glossary of geology, 5th Edition. American Geological Institute, Alexandria, 779 p."@en ;
                                                                        rdfs:comment "Process of melting involving only some of the mineral phases in a rock, to produce a mixture of melt and residual particles."@en ;
                                                                        rdfs:label "partial melting"@en .


###  http://loop3d.org/GSO/ontology/2020/1/geologicprocess/Physical_Weathering
<http://loop3d.org/GSO/ontology/2020/1/geologicprocess/Physical_Weathering> rdf:type owl:Class ;
                                                                            rdfs:subClassOf <http://loop3d.org/GSO/ontology/2020/1/geologicprocess/Weathering> ;
                                                                            <http://purl.org/dc/terms/source> "Neuendorf, K.K.E, Mehl, J.P. & Jackson, J.A. (eds), 2005. Glossary of geology, 5th Edition. American Geological Institute, Alexandria, 779 p."@en ;
                                                                            rdfs:comment "The process of weathering by which frost action, salt-crystal growth, absorption of water, and other physical processes break down a rock to fragments, involving no chemical change"@en ;
                                                                            rdfs:label "physical weathering"@en .


###  http://loop3d.org/GSO/ontology/2020/1/geologicprocess/Plinian_Eruption
<http://loop3d.org/GSO/ontology/2020/1/geologicprocess/Plinian_Eruption> rdf:type owl:Class ;
                                                                         rdfs:subClassOf <http://loop3d.org/GSO/ontology/2020/1/geologicprocess/Pyroclastic_Eruption> ;
                                                                         <http://purl.org/dc/terms/source> "Neuendorf, K.K.E, Mehl, J.P. & Jackson, J.A. (eds), 2005. Glossary of geology, 5th Edition. American Geological Institute, Alexandria, 779 p."@en ;
                                                                         rdfs:comment "An explosive eruption in which a steady, turbulent stream of fragmented magma and magmatic gas is released at a high velocity from a vent. Large volumes of tephra and tall eruption columns are characteristic"@en ;
                                                                         rdfs:label "plinian eruption"@en .


###  http://loop3d.org/GSO/ontology/2020/1/geologicprocess/Polar_Wander
<http://loop3d.org/GSO/ontology/2020/1/geologicprocess/Polar_Wander> rdf:type owl:Class ;
                                                                     rdfs:subClassOf <http://loop3d.org/GSO/ontology/2020/1/geologicprocess/Geomagnetic_Process> ,
                                                                                     <http://loop3d.org/GSO/ontology/2020/1/geology/Transformation> ;
                                                                     <http://purl.org/dc/terms/source> "this vocabulary"@en ;
                                                                     rdfs:comment "Process of migration of the axis of the earth's dipole field relative to the rotation axis of the Earth."@en ;
                                                                     rdfs:label "polar wander"@en .


###  http://loop3d.org/GSO/ontology/2020/1/geologicprocess/Pressure_Release_Weathering
<http://loop3d.org/GSO/ontology/2020/1/geologicprocess/Pressure_Release_Weathering> rdf:type owl:Class ;
                                                                                    rdfs:subClassOf <http://loop3d.org/GSO/ontology/2020/1/geologicprocess/Physical_Weathering> ;
                                                                                    <http://purl.org/dc/terms/source> "Neuendorf, K.K.E, Mehl, J.P. & Jackson, J.A. (eds), 2005. Glossary of geology, 5th Edition. American Geological Institute, Alexandria, 779 p."@en ;
                                                                                    rdfs:comment "Propagation of fractures near the surface of solid rock due to expansion related to release of confining pressure when deeply buried rock is unroofed. Fractures typically propagate along surfaces close to and subparallel to the surface of the outcrop."@en ;
                                                                                    rdfs:label "pressure release weathering"@en .


###  http://loop3d.org/GSO/ontology/2020/1/geologicprocess/Pyroclastic_Eruption
<http://loop3d.org/GSO/ontology/2020/1/geologicprocess/Pyroclastic_Eruption> rdf:type owl:Class ;
                                                                             rdfs:subClassOf <http://loop3d.org/GSO/ontology/2020/1/geologicprocess/Eruption_Process> ;
                                                                             <http://purl.org/dc/terms/source> "Orton, G.J., 1996. Volcanic environments. 485-567 in Readingh.G. (ed.), Sedimentary Environments: Processes, Facies and Stratigraphy, Third Edition. Blackwell Science, Oxford"@en ;
                                                                             rdfs:comment "Eruption produced by the generation and rapid expansion of a gas phase that disrupts magma, surrounding wall rock or sediment"@en ;
                                                                             rdfs:label "pyroclastic eruption"@en .


###  http://loop3d.org/GSO/ontology/2020/1/geologicprocess/Pyrometamorphism
<http://loop3d.org/GSO/ontology/2020/1/geologicprocess/Pyrometamorphism> rdf:type owl:Class ;
                                                                         rdfs:subClassOf <http://loop3d.org/GSO/ontology/2020/1/geologicprocess/Metamorphic_Process> ;
                                                                         rdfs:comment "metamorphism caused by high-temperature near surface events like lightning strikes,  underground coal fires or nuclear reactions."@en ;
                                                                         rdfs:label "Pyrometamorphism "@en .


###  http://loop3d.org/GSO/ontology/2020/1/geologicprocess/Regional_Metamorphism
<http://loop3d.org/GSO/ontology/2020/1/geologicprocess/Regional_Metamorphism> rdf:type owl:Class ;
                                                                              rdfs:subClassOf <http://loop3d.org/GSO/ontology/2020/1/geologicprocess/Metamorphic_Process> ;
                                                                              <http://purl.org/dc/terms/source> "based on Smulikowski et al, 2003"@en ;
                                                                              rdfs:comment "Metamorphic processes driven by temperature and pressure changes affecting a large rock volume, associated with large-scale tectonic processes."@en ;
                                                                              rdfs:label "regional metamorphic genesis"@en .


###  http://loop3d.org/GSO/ontology/2020/1/geologicprocess/Rifting
<http://loop3d.org/GSO/ontology/2020/1/geologicprocess/Rifting> rdf:type owl:Class ;
                                                                rdfs:subClassOf <http://loop3d.org/GSO/ontology/2020/1/geologicprocess/Continental_Breakup> ;
                                                                <http://purl.org/dc/terms/source> "Neuendorf, K.K.E, Mehl, J.P. & Jackson, J.A. (eds), 2005. Glossary of geology, 5th Edition. American Geological Institute, Alexandria, 779 p."@en ;
                                                                rdfs:comment "Extension of the crust to form one or more long, narrow graben of regional extent."@en ;
                                                                rdfs:label "rifting"@en .


###  http://loop3d.org/GSO/ontology/2020/1/geologicprocess/Rock_Forming_Process
<http://loop3d.org/GSO/ontology/2020/1/geologicprocess/Rock_Forming_Process> rdf:type owl:Class ;
                                                                             rdfs:subClassOf <http://loop3d.org/GSO/ontology/2020/1/geology/Geologic_Process> ;
                                                                             rdfs:comment "A process that produces a new igneous or sedimentary rock material. " ;
                                                                             rdfs:label "Rock forming process "@en .


###  http://loop3d.org/GSO/ontology/2020/1/geologicprocess/Sea_Level_Fluctuation
<http://loop3d.org/GSO/ontology/2020/1/geologicprocess/Sea_Level_Fluctuation> rdf:type owl:Class ;
                                                                              rdfs:subClassOf <http://loop3d.org/GSO/ontology/2020/1/hydrology/Hydrologic_Process> ;
                                                                              rdfs:comment "process of alteration of global sea levels due to changes in either the volume of water in the world's oceans or net changes in the volume of the oceanic basins."@en ;
                                                                              rdfs:label "Sea Level Fluctuation"@en .


###  http://loop3d.org/GSO/ontology/2020/1/geologicprocess/Sedimentary_Process
<http://loop3d.org/GSO/ontology/2020/1/geologicprocess/Sedimentary_Process> rdf:type owl:Class ;
                                                                            rdfs:subClassOf <http://loop3d.org/GSO/ontology/2020/1/geology/Geologic_Process> ;
                                                                            <http://purl.org/dc/terms/source> "this vocabulary"@en ;
                                                                            rdfs:comment "A process that changes the distribution or physical properties of sediment at or near the earth's surface"@en ;
                                                                            rdfs:label "Sedimentary Process"@en .


###  http://loop3d.org/GSO/ontology/2020/1/geologicprocess/Shearing
<http://loop3d.org/GSO/ontology/2020/1/geologicprocess/Shearing> rdf:type owl:Class ;
                                                                 rdfs:subClassOf <http://loop3d.org/GSO/ontology/2020/1/geology/Deformation> ;
                                                                 <http://purl.org/dc/terms/source> "Neuendorf, K.K.E, Mehl, J.P. & Jackson, J.A. (eds), 2005. Glossary of geology, 5th Edition. American Geological Institute, Alexandria, 779 p."@en ;
                                                                 rdfs:comment "A deformation in which contiguous parts of a body are displaced relatively to each other in a direction parallel to a surface. The surface may be a discrete fault, or the deformation may be a penetrative strain and the shear surface is a geometric abstraction."@en ;
                                                                 rdfs:label "shearing"@en .


###  http://loop3d.org/GSO/ontology/2020/1/geologicprocess/Speciation
<http://loop3d.org/GSO/ontology/2020/1/geologicprocess/Speciation> rdf:type owl:Class ;
                                                                   rdfs:subClassOf <http://loop3d.org/GSO/ontology/2020/1/geologicprocess/Biological_Process> ;
                                                                   <http://purl.org/dc/terms/source> "this vocabulary"@en ;
                                                                   rdfs:comment "process that results inappearance of new species"@en ;
                                                                   rdfs:label "speciation"@en .


###  http://loop3d.org/GSO/ontology/2020/1/geologicprocess/Spreading
<http://loop3d.org/GSO/ontology/2020/1/geologicprocess/Spreading> rdf:type owl:Class ;
                                                                  rdfs:subClassOf <http://loop3d.org/GSO/ontology/2020/1/geologicprocess/Tectonic_Process> ,
                                                                                  <http://loop3d.org/GSO/ontology/2020/1/geology/Additive_Process> ,
                                                                                  <http://loop3d.org/GSO/ontology/2020/1/geology/Deformation> ;
                                                                  <http://purl.org/dc/terms/source> "Neuendorf, K.K.E, Mehl, J.P. & Jackson, J.A. (eds), 2005. Glossary of geology, 5th Edition. American Geological Institute, Alexandria, 779 p."@en ;
                                                                  rdfs:comment "A process whereby new oceanic crust is formed by upwelling of magma at the center of mid-ocean ridges and by a moving-away of the new material from the site of upwelling at rates of one to ten centimeters per year."@en ;
                                                                  rdfs:label "spreading"@en .


###  http://loop3d.org/GSO/ontology/2020/1/geologicprocess/Strombolian_Eruption
<http://loop3d.org/GSO/ontology/2020/1/geologicprocess/Strombolian_Eruption> rdf:type owl:Class ;
                                                                             rdfs:subClassOf <http://loop3d.org/GSO/ontology/2020/1/geologicprocess/Eruption_Process> ;
                                                                             <http://purl.org/dc/terms/source> "Neuendorf, K.K.E, Mehl, J.P. & Jackson, J.A. (eds), 2005. Glossary of geology, 5th Edition. American Geological Institute, Alexandria, 779 p."@en ;
                                                                             rdfs:comment "Eruption characterized by jetting of clots or \\fountains\\ of fluid, basaltic lava from a central crater"@en ;
                                                                             rdfs:label "strombolian eruption"@en .


###  http://loop3d.org/GSO/ontology/2020/1/geologicprocess/Subaerial_Extrusion
<http://loop3d.org/GSO/ontology/2020/1/geologicprocess/Subaerial_Extrusion> rdf:type owl:Class ;
                                                                            rdfs:subClassOf <http://loop3d.org/GSO/ontology/2020/1/geologicprocess/Eruption_Process> ;
                                                                            <http://purl.org/dc/terms/source> "This vocabulary"@en ;
                                                                            rdfs:comment "Process of magma crystallisation either in the open air or immediately adjacent to the land surface."@en ;
                                                                            rdfs:label "subaerial extrusion"@en .


###  http://loop3d.org/GSO/ontology/2020/1/geologicprocess/Subaqueous_Extrusion
<http://loop3d.org/GSO/ontology/2020/1/geologicprocess/Subaqueous_Extrusion> rdf:type owl:Class ;
                                                                             rdfs:subClassOf <http://loop3d.org/GSO/ontology/2020/1/geologicprocess/Eruption_Process> ;
                                                                             <http://purl.org/dc/terms/source> "This vocabulary"@en ;
                                                                             rdfs:comment "Process of magma crystallisation under water or ice."@en ;
                                                                             rdfs:label "subaqueous extrusion"@en .


###  http://loop3d.org/GSO/ontology/2020/1/geologicprocess/Subduction
<http://loop3d.org/GSO/ontology/2020/1/geologicprocess/Subduction> rdf:type owl:Class ;
                                                                   rdfs:subClassOf <http://loop3d.org/GSO/ontology/2020/1/geologicprocess/Tectonic_Process> ,
                                                                                   <http://loop3d.org/GSO/ontology/2020/1/geology/Deformation> ,
                                                                                   <http://loop3d.org/GSO/ontology/2020/1/geology/Subtractive_Process> ;
                                                                   <http://purl.org/dc/terms/source> "Neuendorf, K.K.E, Mehl, J.P. & Jackson, J.A. (eds), 2005. Glossary of geology, 5th Edition. American Geological Institute, Alexandria, 779 p."@en ;
                                                                   rdfs:comment "The process of one lithospheric plate descending beneath another"@en ;
                                                                   rdfs:label "subduction"@en .


###  http://loop3d.org/GSO/ontology/2020/1/geologicprocess/Tectonic_Process
<http://loop3d.org/GSO/ontology/2020/1/geologicprocess/Tectonic_Process> rdf:type owl:Class ;
                                                                         rdfs:subClassOf <http://loop3d.org/GSO/ontology/2020/1/geology/Geologic_Process> ;
                                                                         <http://purl.org/dc/terms/source> "this vocabulary"@en ;
                                                                         rdfs:comment "Processes related to the interaction between or deformation of rigid plates forming the crust of the Earth."@en ;
                                                                         rdfs:label "Tectonic Process"@en .


###  http://loop3d.org/GSO/ontology/2020/1/geologicprocess/Thermal_Shock_Weathering
<http://loop3d.org/GSO/ontology/2020/1/geologicprocess/Thermal_Shock_Weathering> rdf:type owl:Class ;
                                                                                 rdfs:subClassOf <http://loop3d.org/GSO/ontology/2020/1/geologicprocess/Physical_Weathering> ;
                                                                                 <http://purl.org/dc/terms/source> "this vocabulary"@en ;
                                                                                 rdfs:comment "Propagation of fractures near the surface of solid rock due to expansion and contraction caused by temperature changes. Fractures typically propagate along surfaces close to and subparallel to the surface of the outcrop."@en ;
                                                                                 rdfs:label "thermal shock weathering"@en .


###  http://loop3d.org/GSO/ontology/2020/1/geologicprocess/Traction_Saltation_or_Suspension_Deposition
<http://loop3d.org/GSO/ontology/2020/1/geologicprocess/Traction_Saltation_or_Suspension_Deposition> rdf:type owl:Class ;
                                                                                                    rdfs:subClassOf <http://loop3d.org/GSO/ontology/2020/1/geologicprocess/Mechanical_Deposition> ;
                                                                                                    <http://purl.org/dc/terms/source> "this vocabulary"@en ;
                                                                                                    rdfs:comment "Deposition of sediment from moving water or air, in which the sediment is transported by entrainment in the moving fluid. Constrast with debris flow or turbidity current deposition in which movement of fluid/sediment mixture is due to incorporation of sediment in fluid."@en ;
                                                                                                    rdfs:label "deposition from moving fluid"@en .


###  http://loop3d.org/GSO/ontology/2020/1/geologicprocess/Transform_Faulting
<http://loop3d.org/GSO/ontology/2020/1/geologicprocess/Transform_Faulting> rdf:type owl:Class ;
                                                                           rdfs:subClassOf <http://loop3d.org/GSO/ontology/2020/1/geologicprocess/Faulting> ,
                                                                                           <http://loop3d.org/GSO/ontology/2020/1/geologicprocess/Tectonic_Process> ;
                                                                           <http://purl.org/dc/terms/source> "Neuendorf, K.K.E, Mehl, J.P. & Jackson, J.A. (eds), 2005. Glossary of geology, 5th Edition. American Geological Institute, Alexandria, 779 p."@en ;
                                                                           rdfs:comment "A strike-slip fault that links two other faults or two other plate boundaries (e.g. two segments of a mid-ocean ridge). Transform faults often exhibit characteristics that distinguish them from transcurrent faults: (1) For transform faults formed at the same time as the faults they link, slip on the transform fault has equal magnitude at all points along the transform, slip magnitude on the transform fault can exceed the length of the transform fault, and slip does not decrease to zero at the fault termini. (2) For transform faults linking two similar features, e.g. if two mid-ocean ridge segments linked by a transform have equal spreading rates, then the length of the transform does not change as slip accrues on it."@en ;
                                                                           rdfs:label "transform faulting"@en .


###  http://loop3d.org/GSO/ontology/2020/1/geologicprocess/Turbidity_Current_Deposition
<http://loop3d.org/GSO/ontology/2020/1/geologicprocess/Turbidity_Current_Deposition> rdf:type owl:Class ;
                                                                                     rdfs:subClassOf <http://loop3d.org/GSO/ontology/2020/1/geologicprocess/Mechanical_Deposition> ;
                                                                                     <http://purl.org/dc/terms/source> "Postma 1986 Geology v. 14 p291-294"@en ;
                                                                                     rdfs:comment "Deposition from a turbulent, low concentration sediment-water mixture."@en ;
                                                                                     rdfs:label "turbidity current deposition"@en .


###  http://loop3d.org/GSO/ontology/2020/1/geologicprocess/Vulcanian_Eruption
<http://loop3d.org/GSO/ontology/2020/1/geologicprocess/Vulcanian_Eruption> rdf:type owl:Class ;
                                                                           rdfs:subClassOf <http://loop3d.org/GSO/ontology/2020/1/geologicprocess/Pyroclastic_Eruption> ;
                                                                           <http://purl.org/dc/terms/source> "Neuendorf, K.K.E, Mehl, J.P. & Jackson, J.A. (eds), 2005. Glossary of geology, 5th Edition. American Geological Institute, Alexandria, 779 p."@en ;
                                                                           rdfs:comment "Eruption characterized by the explosive ejection of fragments of new lava, commonly incandescent when they leave the vent but either solid or too viscous to assume any appreciable degree of rounding during their flight through the air. With these there are often breadcrust bombs or blocks, and generally large proportions of ash"@en ;
                                                                           rdfs:label "vulcanian eruption"@en .


###  http://loop3d.org/GSO/ontology/2020/1/geologicprocess/Water_Erosion
<http://loop3d.org/GSO/ontology/2020/1/geologicprocess/Water_Erosion> rdf:type owl:Class ;
                                                                      rdfs:subClassOf <http://loop3d.org/GSO/ontology/2020/1/geologicprocess/Erosion> ;
                                                                      <http://purl.org/dc/terms/source> "this vocabulary"@en ;
                                                                      rdfs:comment "Erosion by clast impact or plucking by moving liquid water"@en ;
                                                                      rdfs:label "water erosion"@en .


###  http://loop3d.org/GSO/ontology/2020/1/geologicprocess/Weathering
<http://loop3d.org/GSO/ontology/2020/1/geologicprocess/Weathering> rdf:type owl:Class ;
                                                                   rdfs:subClassOf <http://loop3d.org/GSO/ontology/2020/1/geology/Transformation> ;
                                                                   <http://purl.org/dc/terms/source> "this vocabulary"@en ;
                                                                   rdfs:comment "The process or group of processes by which earth materials exposed to atmospheric agents at or near the Earth's surface are changed in color, texture, composition, firmness, or form, with little or no transport of the loosened or altered material. Processes typically include oxidationhydration, and leaching of soluble constituents."@en ;
                                                                   rdfs:label "weathering"@en .


###  http://loop3d.org/GSO/ontology/2020/1/geologicprocess/Wind_Erosion
<http://loop3d.org/GSO/ontology/2020/1/geologicprocess/Wind_Erosion> rdf:type owl:Class ;
                                                                     rdfs:subClassOf <http://loop3d.org/GSO/ontology/2020/1/geologicprocess/Erosion> ;
                                                                     <http://purl.org/dc/terms/source> "this vocabulary"@en ;
                                                                     rdfs:comment "Erosion by clast impact or plucking by moving air (wind)"@en ;
                                                                     rdfs:label "wind erosion"@en .


###  http://loop3d.org/GSO/ontology/2020/1/geology/Additive_Process
<http://loop3d.org/GSO/ontology/2020/1/geology/Additive_Process> rdf:type owl:Class .


###  http://loop3d.org/GSO/ontology/2020/1/geology/Deformation
<http://loop3d.org/GSO/ontology/2020/1/geology/Deformation> rdf:type owl:Class .


###  http://loop3d.org/GSO/ontology/2020/1/geology/Geologic_Process
<http://loop3d.org/GSO/ontology/2020/1/geology/Geologic_Process> rdf:type owl:Class .


###  http://loop3d.org/GSO/ontology/2020/1/geology/Subtractive_Process
<http://loop3d.org/GSO/ontology/2020/1/geology/Subtractive_Process> rdf:type owl:Class .


###  http://loop3d.org/GSO/ontology/2020/1/geology/Transformation
<http://loop3d.org/GSO/ontology/2020/1/geology/Transformation> rdf:type owl:Class .


###  http://loop3d.org/GSO/ontology/2020/1/hydrology/Hydrologic_Process
<http://loop3d.org/GSO/ontology/2020/1/hydrology/Hydrologic_Process> rdf:type owl:Class .


###  http://org.semanticweb.owlapi/error#Error1
<http://org.semanticweb.owlapi/error#Error1> rdf:type owl:Class .


[ owl:qualifiedCardinality "1"^^xsd:nonNegativeInteger
] .

###  Generated by the OWL API (version 5.1.14) https://github.com/owlcs/owlapi/
